src/dvspec/dafny/att_spec_proofs/dvn_next_inv.dfy
@@ -21,27 +21,33 @@ module DVN_Next_Inv
     import opened Fnc_Inv
     import opened Helper_Sets_Lemmas
 
-    lemma lemma_dvn_next_inv1(dvn: DVState, dvn': DVState)       
+    lemma lemma_inv1_dvn_next(dvn: DVState, dvn': DVState)       
     requires exists e: DV.Event :: DV.NextEvent(dvn, e, dvn')
     requires inv1(dvn)
     ensures inv1(dvn')
     { }
 
-    lemma lemma_dvn_next_inv2(dvn: DVState, dvn': DVState)       
+    lemma lemma_inv2_dvn_next(dvn: DVState, dvn': DVState)       
     requires exists e: DV.Event :: DV.NextEvent(dvn, e, dvn')
     requires inv2(dvn)
     ensures inv2(dvn')
     { }
 
-    lemma lemma_dvn_next_inv3(
+    lemma lemma_inv3_dvn_next(dvn: DVState, dvn': DVState)       
+    requires exists e: DV.Event :: DV.NextEvent(dvn, e, dvn')
+    requires inv3(dvn)
+    ensures inv3(dvn')
+    { }
+
+    lemma lemma_inv4_dvn_next(
         dvn: DVState,
         event: DV.Event,
         dvn': DVState
     )
-    requires inv1(dvn)
+    requires inv1(dvn)    
     requires NextEvent(dvn, event, dvn')
-    requires inv3(dvn)
-    ensures inv3(dvn')
+    requires inv4(dvn)
+    ensures inv4(dvn')
     {        
         match event 
         {
@@ -78,13 +84,17 @@ module DVN_Next_Inv
                                     var k: nat :| && k < dvn.index_next_attestation_duty_to_be_served
                                                   && dvn.sequence_attestation_duties_to_be_served[k].node == hn
                                                   && dvn.sequence_attestation_duties_to_be_served[k].attestation_duty == duty;
+
+                                    assert && k < dvn'.index_next_attestation_duty_to_be_served
+                                           && dvn'.sequence_attestation_duties_to_be_served[k].node == hn
+                                           && dvn'.sequence_attestation_duties_to_be_served[k].attestation_duty == duty;
                                 }
                             }
                             else 
                             {                                   
                                 var curr_index := dvn.index_next_attestation_duty_to_be_served;
                                 var new_duty := dvn.sequence_attestation_duties_to_be_served[curr_index].attestation_duty;
-                                lemma_f_serve_attestation_duty_inv3(dvc, new_duty, dvc');    
+                                lemma_inv4_f_serve_attestation_duty(dvc, new_duty, dvc');    
                                 assert dvc'.all_rcvd_duties == dvc.all_rcvd_duties + {new_duty};                                                            
                                 assert new_duty in dvc'.all_rcvd_duties;                                                          
 
@@ -106,6 +116,10 @@ module DVN_Next_Inv
                                         var k: nat :| && k < dvn.index_next_attestation_duty_to_be_served
                                                       && dvn.sequence_attestation_duties_to_be_served[k].node == hn
                                                       && dvn.sequence_attestation_duties_to_be_served[k].attestation_duty == duty;                                        
+                                        
+                                        assert && k < dvn'.index_next_attestation_duty_to_be_served
+                                               && dvn'.sequence_attestation_duties_to_be_served[k].node == hn
+                                               && dvn'.sequence_attestation_duties_to_be_served[k].attestation_duty == duty;
                                     }
                                 }      
                                                    
@@ -113,14 +127,14 @@ module DVN_Next_Inv
                         }                        
                         
                     case AttConsensusDecided(id, decided_attestation_data) => 
-                        lemma_f_att_consensus_decided_inv3(dvc, id, decided_attestation_data, dvc');                        
+                        lemma_inv4_f_att_consensus_decided(dvc, id, decided_attestation_data, dvc');                        
                         
                     case ReceviedAttesttionShare(attestation_share) =>                         
-                        lemma_f_listen_for_attestation_shares_inv3(dvc, attestation_share, dvc');                        
+                        lemma_inv4_f_listen_for_attestation_shares(dvc, attestation_share, dvc');                        
    
                     case ImportedNewBlock(block) => 
                         var dvc := add_block_to_bn(dvc, nodeEvent.block);
-                        lemma_f_listen_for_new_imported_blocks_inv3(dvc, block, dvc');                        
+                        lemma_inv4_f_listen_for_new_imported_blocks(dvc, block, dvc');                        
                                                 
                     case ResendAttestationShares =>                         
                         
@@ -133,6 +147,43 @@ module DVN_Next_Inv
         }        
     }   
     
-    
- 
+    lemma lemma_inv5_dvn_next(
+        dvn: DVState,
+        event: DV.Event,
+        dvn': DVState
+    )    
+    requires NextEvent(dvn, event, dvn')
+    requires inv5(dvn)
+    ensures inv5(dvn')
+    {        
+        match event 
+        {
+            case HonestNodeTakingStep(node, nodeEvent, nodeOutputs) =>
+                var dvc := dvn.honest_nodes_states[node];
+                var dvc' := dvn'.honest_nodes_states[node];
+                match nodeEvent
+                {
+                    case ServeAttstationDuty(attestation_duty) =>     
+                        lemma_inv5_f_serve_attestation_duty(dvc, attestation_duty, dvc');
+                        
+                    case AttConsensusDecided(id, decided_attestation_data) => 
+                        lemma_inv5_f_att_consensus_decided(dvc, id, decided_attestation_data, dvc');                        
+                        
+                    case ReceviedAttesttionShare(attestation_share) =>                         
+                        lemma_inv5_f_listen_for_attestation_shares(dvc, attestation_share, dvc');                        
+   
+                    case ImportedNewBlock(block) => 
+                        var dvc := add_block_to_bn(dvc, nodeEvent.block);
+                        lemma_inv5_f_listen_for_new_imported_blocks(dvc, block, dvc');                        
+                                                
+                    case ResendAttestationShares =>                         
+                        
+                    case NoEvent => 
+                        
+                }
+
+            case AdeversaryTakingStep(node, new_attestation_share_sent, messagesReceivedByTheNode) =>
+                
+        }   
+    }
 }
